arm+riscv64 access: proof update for access control changes
Signed-off-by: Ryan Barry <ryan.barry@proofcraft.systems>

proof/access-control/RISCV64/ArchAccess.thy
@@ -8,7 +8,7 @@ theory ArchAccess
 imports Types
 begin
 
-context Arch begin global_naming RISCV64
+context Arch begin arch_global_naming
 
 subsection \<open>Arch-specific transformation of caps into authorities\<close>
 
@@ -46,43 +46,6 @@ definition state_vrefs where
   "state_vrefs s \<equiv> \<lambda>p.
      \<Union>{vs_refs_aux lvl ao | lvl ao bot asid vref. vs_lookup_table bot asid vref s = Some (lvl, p)
                                                    \<and> aobjs_of s p = Some ao \<and> vref \<in> user_region}"
-
-lemma state_vrefsD:
-  "\<lbrakk> vs_lookup_table level asid vref s = Some (lvl, p);
-     aobjs_of s p = Some ao; vref \<in> user_region; x \<in> vs_refs_aux lvl ao \<rbrakk>
-     \<Longrightarrow> x \<in> state_vrefs s p"
-  unfolding state_vrefs_def by fastforce
-
-end
-
-context Arch_p_arch_update_eq begin global_naming RISCV64
-
-interpretation Arch .
-
-lemma state_vrefs[iff]: "state_vrefs (f s) = state_vrefs s"
-  by (simp add: state_vrefs_def pspace)
-
-end
-
-context Arch begin global_naming RISCV64
-
-lemmas state_vrefs_upd =
-  cur_thread_update.state_vrefs
-  cdt_update.state_vrefs
-  irq_node_update_arch.state_vrefs
-  interrupt_update.state_vrefs
-  revokable_update.state_vrefs
-  machine_state_update.state_vrefs
-  more_update.state_vrefs
-  scheduler_action_update.state_vrefs
-  domain_index_update.state_vrefs
-  cur_domain_update.state_vrefs
-  domain_time_update.state_vrefs
-  ready_queues_update.state_vrefs
-
-end
-
-context Arch begin
 
 primrec aobj_ref' where
   "aobj_ref' (ASIDPoolCap p as) = {p}"
@@ -122,104 +85,50 @@ section \<open>Arch-specific integrity definition\<close>
 
 subsection \<open>How ASIDs can change\<close>
 
-abbreviation integrity_asids_aux :: "'a PAS \<Rightarrow> 'a set \<Rightarrow> obj_ref \<Rightarrow> asid \<Rightarrow>
-                                     (asid_high_index \<rightharpoonup> obj_ref) \<Rightarrow> (asid_high_index \<rightharpoonup> obj_ref) \<Rightarrow>
-                                     (obj_ref \<rightharpoonup> asid_pool) \<Rightarrow> (obj_ref \<rightharpoonup> asid_pool) \<Rightarrow> bool" where
-  "integrity_asids_aux aag subjects x asid atab atab' pools pools'  \<equiv>
-     (atab (asid_high_bits_of asid) \<noteq> atab' (asid_high_bits_of asid)
-      \<longrightarrow> (\<forall>x. atab' (asid_high_bits_of asid) = Some x \<longrightarrow> pasObjectAbs aag x \<in> subjects) \<and>
+definition integrity_asids_2 ::
+  "'a PAS \<Rightarrow> 'a set \<Rightarrow> obj_ref \<Rightarrow> asid \<Rightarrow> arch_state \<Rightarrow> arch_state \<Rightarrow>
+   (obj_ref \<rightharpoonup> arch_kernel_obj) \<Rightarrow> (obj_ref \<rightharpoonup> arch_kernel_obj) \<Rightarrow> bool"
+where
+  "integrity_asids_2 aag subjects x asid as as' ao ao'  \<equiv>
+     (riscv_asid_table as (asid_high_bits_of asid) \<noteq> riscv_asid_table as' (asid_high_bits_of asid)
+      \<longrightarrow> (\<forall>x. riscv_asid_table as' (asid_high_bits_of asid) = Some x \<longrightarrow> pasObjectAbs aag x \<in> subjects) \<and>
           (\<forall>asid'. asid' \<noteq> 0 \<and> asid_high_bits_of asid' = asid_high_bits_of asid
                    \<longrightarrow> pasASIDAbs aag asid' \<in> subjects)) \<and>
      (pasObjectAbs aag x \<notin> subjects
-      \<longrightarrow> (\<forall>pool. pools x = Some pool
-                  \<longrightarrow> pools' x \<noteq> None \<and>
-                      (\<forall>pool'. pools' x = Some pool' \<longrightarrow>
-                               (pool \<noteq> pool' \<longrightarrow> (\<exists>asid. atab (asid_high_bits_of asid) = Some x)))))"
+      \<longrightarrow> (\<forall>pool. (ao |> asid_pool_of) x = Some pool
+                  \<longrightarrow> (ao' |> asid_pool_of) x \<noteq> None \<and>
+                      (\<forall>pool'. (ao' |> asid_pool_of) x = Some pool' \<longrightarrow>
+                               (pool \<noteq> pool' \<longrightarrow> (\<exists>asid. riscv_asid_table as (asid_high_bits_of asid) = Some x)))))"
 
-definition integrity_asids ::
-  "'a PAS \<Rightarrow> 'a set \<Rightarrow> obj_ref \<Rightarrow> asid \<Rightarrow> 'y::state_ext state \<Rightarrow> 'z::state_ext state  \<Rightarrow> bool" where
-  "integrity_asids aag subjects x asid s s' \<equiv>
-   integrity_asids_aux aag subjects x asid (asid_table s) (asid_table s')
-                                           (asid_pools_of s) (asid_pools_of s')"
+lemmas integrity_asids_def = integrity_asids_2_def
 
-sublocale kheap_update: Arch_arch_update_eq "kheap_update f"
-  by unfold_locales simp
+\<comment> \<open>No hypervisor\<close>
+definition integrity_hyp_2 ::
+  "'a PAS \<Rightarrow> 'a set \<Rightarrow> obj_ref \<Rightarrow> machine_state \<Rightarrow> machine_state \<Rightarrow> arch_state \<Rightarrow> arch_state
+          \<Rightarrow> (obj_ref \<Rightarrow> arch_kernel_obj option) \<Rightarrow> (obj_ref \<Rightarrow> arch_kernel_obj option) \<Rightarrow> bool"
+where
+  "integrity_hyp_2 aag subjects x ms ms' as as' aobjs aobjs' \<equiv> True"
 
-lemma (in Arch_p_arch_update_eq) integrity_asids_update[simp]:
-  "integrity_asids aag subjects x a (f st) s = integrity_asids aag subjects x a st s"
-  "integrity_asids aag subjects x a st (f s) = integrity_asids aag subjects x a st s"
-  by (auto simp: integrity_asids_def arch pspace)
+lemmas integrity_hyp_def = integrity_hyp_2_def
 
-lemmas integrity_asids_updates =
-  cdt_update.integrity_asids_update
-  more_update.integrity_asids_update
-  revokable_update.integrity_asids_update
-  interrupt_update.integrity_asids_update
-  cur_thread_update.integrity_asids_update
-  machine_state_update.integrity_asids_update
-  scheduler_action_update.integrity_asids_update
-  domain_index_update.integrity_asids_update
-  cur_domain_update.integrity_asids_update
-  domain_time_update.integrity_asids_update
-  ready_queues_update.integrity_asids_update
+definition valid_cur_hyp :: "'s::state_ext state \<Rightarrow> bool" where
+  "valid_cur_hyp \<equiv> \<top>"
 
-lemma integrity_asids_cnode_update':
-  "\<lbrakk> kheap st p = Some (CNode sz cs); integrity_asids aag subjects x a st (s\<lparr>kheap := rest\<rparr>) \<rbrakk>
-     \<Longrightarrow> integrity_asids aag subjects x a st (s\<lparr>kheap := \<lambda>x. if x = p then v else rest x\<rparr>)"
-  by (auto simp: integrity_asids_def opt_map_def split: option.splits)
+\<comment> \<open>No FPU\<close>
+definition integrity_fpu_2 ::
+  "'a PAS \<Rightarrow> 'a set \<Rightarrow> obj_ref \<Rightarrow> machine_state \<Rightarrow> machine_state
+          \<Rightarrow> (obj_ref \<Rightarrow> kernel_object option) \<Rightarrow> (obj_ref \<Rightarrow> kernel_object option) \<Rightarrow> bool"
+where
+  "integrity_fpu_2 aag subjects x ms ms' kh kh' \<equiv> True"
 
-lemma integrity_asids_tcb_update':
-  "\<lbrakk> kheap st p = Some (TCB tcb); integrity_asids aag subjects x a st (s\<lparr>kheap := rest\<rparr>) \<rbrakk>
-     \<Longrightarrow> integrity_asids aag subjects x a st (s\<lparr>kheap := \<lambda>x. if x = p then v else rest x\<rparr>)"
-  by (auto simp: integrity_asids_def opt_map_def split: option.splits)
-
-lemma integrity_asids_ep_update':
-  "\<lbrakk> kheap st p = Some (Endpoint ep); integrity_asids aag subjects x a st (s\<lparr>kheap := rest\<rparr>) \<rbrakk>
-     \<Longrightarrow> integrity_asids aag subjects x a st (s\<lparr>kheap := \<lambda>x. if x = p then v else rest x\<rparr>)"
-  by (auto simp: integrity_asids_def opt_map_def split: option.splits)
-
-lemma integrity_asids_ntfn_update':
-  "\<lbrakk> kheap st p = Some (Notification ntfn); integrity_asids aag subjects x a st (s\<lparr>kheap := rest\<rparr>) \<rbrakk>
-     \<Longrightarrow> integrity_asids aag subjects x a st (s\<lparr>kheap := \<lambda>x. if x = p then v else rest x\<rparr>)"
-  by (auto simp: integrity_asids_def opt_map_def split: option.splits)
-
-lemmas integrity_asids_kh_upds'' =
-  integrity_asids_cnode_update'
-  integrity_asids_tcb_update'
-  integrity_asids_ep_update'
-  integrity_asids_ntfn_update'
-
-lemmas integrity_asids_kh_upds =
-  integrity_asids_kh_upds''
-  integrity_asids_kh_upds''[where rest="kheap s" and s=s for s, folded fun_upd_def, simplified]
-
-declare integrity_asids_def[simp]
-
-lemma integrity_asids_kh_upds':
-  "integrity_asids aag subjects x a (s\<lparr>kheap := (kheap s)(p \<mapsto> CNode sz cs)\<rparr>) s"
-  "integrity_asids aag subjects x a (s\<lparr>kheap := (kheap s)(p \<mapsto> TCB tcb)\<rparr>) s"
-  "integrity_asids aag subjects x a (s\<lparr>kheap := (kheap s)(p \<mapsto> Endpoint ep)\<rparr>) s"
-  "integrity_asids aag subjects x a (s\<lparr>kheap := (kheap s)(p \<mapsto> Notification ntfn)\<rparr>) s"
-  by (auto simp: opt_map_def split: option.splits)
-
-lemma integrity_asids_kh_update:
-  "integrity_asids aag subject x a (s\<lparr>kheap := kh\<rparr>) (s\<lparr>kheap := kh'\<rparr>)
-   \<Longrightarrow> integrity_asids aag subject x a (s\<lparr>kheap := kh(p := v)\<rparr>) (s\<lparr>kheap := kh'(p := v)\<rparr>)"
-  by (clarsimp simp: opt_map_def)
+lemmas integrity_fpu_def = integrity_fpu_2_def
 
 
 subsection \<open>Misc definitions\<close>
 
-fun ctxt_IP_update where
-  "ctxt_IP_update (UserContext ctxt) = UserContext (ctxt(NextIP := ctxt FaultIP))"
-
-lemma ctxt_IP_update_def:
-  "ctxt_IP_update ctxt =
-   (case ctxt of (UserContext ctxt') \<Rightarrow> UserContext (ctxt'(NextIP := ctxt' FaultIP)))"
-  by (cases ctxt; clarsimp)
-
 abbreviation arch_IP_update where
-  "arch_IP_update arch \<equiv> arch_tcb_context_set (ctxt_IP_update (arch_tcb_context_get arch)) arch"
+  "arch_IP_update a \<equiv>
+   arch_tcb_set_registers ((arch_tcb_get_registers a)(NextIP := arch_tcb_get_registers a FaultIP)) a"
 
 definition asid_pool_integrity ::
   "'a set \<Rightarrow> 'a PAS \<Rightarrow> (asid_low_index \<rightharpoonup> obj_ref) \<Rightarrow> (asid_low_index \<rightharpoonup> obj_ref) \<Rightarrow> bool" where
@@ -255,34 +164,5 @@ definition auth_ipc_buffers :: "'z::state_ext state \<Rightarrow> obj_ref \<Righ
       | _ \<Rightarrow> {})"
 
 end
-
-
-context begin interpretation Arch .
-
-requalify_consts
-  vspace_cap_rights_to_auth
-  aobj_ref'
-  acap_asid'
-  state_vrefs
-  state_asids_to_policy_arch
-  integrity_asids
-  ctxt_IP_update
-  arch_IP_update
-  arch_cap_auth_conferred
-  arch_integrity_obj_atomic
-  arch_integrity_obj_alt
-  auth_ipc_buffers
-
-requalify_facts
-  integrity_asids_updates
-  state_vrefs_upd
-  integrity_asids_kh_upds
-  integrity_asids_kh_upds'
-  integrity_asids_kh_update
-
-end
-
-declare state_vrefs_upd[simp]
-declare integrity_asids_updates[simp]
 
 end
