proof/access-control/RISCV64/ArchTcb_AC.thy
@@ -8,13 +8,16 @@ theory ArchTcb_AC
 imports Tcb_AC
 begin
 
-context Arch begin global_naming RISCV64
+context Arch begin arch_global_naming
 
 named_theorems Tcb_AC_assms
 
 declare arch_get_sanitise_register_info_inv[Tcb_AC_assms]
 
-crunch arch_post_modify_registers, arch_post_set_flags
+crunch arch_post_set_flags
+  for inv[Tcb_AC_assms,wp]: P
+
+crunch arch_post_modify_registers
   for pas_refined[Tcb_AC_assms, wp]: "pas_refined aag"
 
 lemma arch_post_modify_registers_respects[Tcb_AC_assms]:
@@ -109,7 +112,7 @@ global_interpretation Tcb_AC_1?: Tcb_AC_1
 proof goal_cases
   interpret Arch .
   case 1 show ?case
-    by (unfold_locales; (fact Tcb_AC_assms)?)
+    by (unfold_locales; (fact Tcb_AC_assms | solves \<open>wp only: Tcb_AC_assms; simp\<close>)?)
 qed
 
 end
